src/FS/Trees.v
@@ -10,7 +10,6 @@ Require Import Morphisms.
 Import ListNotations.
 Open Scope string.
 
-
 (** Data types *)
 
 Inductive Node :=
@@ -87,6 +86,15 @@ Proof.
     etransitivity; eauto.
 Qed.
 
+Ltac subst_fsequiv :=
+  match goal with
+  | H : FSEquiv ?s1 ?s2 |- _ =>
+    idtac "substituting" s1 "using" H; rewrite H in *; clear H; clear s1;
+    idtac "cleared" s1
+  | H : FSEquiv ?s1 ?s2 |- _ =>
+    idtac "substituting" s2 "using" H; rewrite <- H in *; clear H; clear s2;
+    idtac "cleared" s2
+  end.
 
 (** [path_evaluates] is used to specify lookup *)
 
@@ -183,118 +191,826 @@ Proof.
   unfold FSEquiv in *; intuition.
 Qed.
 
-
-(** Largely boilerplate helpers and proof hints *)
-
 Hint Constructors valid_link.
 Hint Constructors path_evaluates.
 
-Hint Extern 1 False =>
+Definition does_not_exist (fs : FS) dirnum name :=
+  ~ exists n, Graph.In (mkLink dirnum n name) (FSLinks fs).
+
+Definition file_handle_unused (fs : FS) h :=
+  ~ exists d name, Graph.In (mkLink d (FileNode h) name) (FSLinks fs).
+
+Definition file_handle_valid (fs : FS) h :=
+  h < Datatypes.length (FSFiles fs).
+
+Definition upd_file h data (fs : FS) :=
+  mkFS (FSRoot fs) (FSLinks fs) (list_upd (FSFiles fs) h data).
+
+Definition add_link dir node name (fs : FS) :=
+  mkFS (FSRoot fs) (Graph.add (mkLink dir node name) (FSLinks fs)) (FSFiles fs).
+
+Definition create_file dir h name (fs : FS) :=
+  add_link dir (FileNode h) name (upd_file h "" fs).
+
+Definition valid_dir dir (fs : FS) :=
+  exists pn, path_eval_root fs pn (DirNode dir).
+
+Definition unique_pathname (fs : FS) pn :=
+  exists node,
+    path_eval_root fs pn node /\
+    forall node',
+      path_eval_root fs pn node' -> node' = node.
+
+Definition unique_dirents (fs : FS) :=
+  forall dir name target target0,
+    valid_link fs dir name target ->
+    valid_link fs dir name target0 ->
+    target0 = target.
+
+Definition fs_invariant (fs : FS) :=
+  unique_dirents fs.
+
+Lemma valid_link_eq: forall fs dir a node node0,
+    fs_invariant fs ->
+    valid_link fs dir a node ->
+    valid_link fs dir a node0 ->
+    node = node0.
+Proof.
+  unfold fs_invariant, unique_dirents in *.
+  intros; eauto.
+Qed.
+
+Lemma path_evaluates_eq: forall pn fs dir node node',
+    fs_invariant fs ->
+    path_evaluates fs dir pn node ->
+    path_evaluates fs dir pn node'->
+    node = node'.
+Proof.
+  intros.
+  generalize dependent node'.
+  induction H0; intros.
+  + inversion H1; subst.
+    inversion H1; subst; auto.
+  + inversion H1; subst.
+    eapply valid_link_eq in H0; eauto.
+    exfalso.
+    eapply valid_link_eq with (node := (DirNode inum0)) in H0; auto.
+    inversion H0.
+    exfalso.
+    eapply valid_link_eq with (node := (SymlinkNode sympath)) in H0; auto.
+    inversion H0.
+  + inversion H2; subst.
+    - exfalso.
+      eapply valid_link_eq with (node := (FileNode inum0)) in H0; auto.
+      inversion H0.
+    - eapply valid_link_eq in H0; eauto.
+      inversion H0; subst.
+      apply IHpath_evaluates; auto.
+    - exfalso.
+      eapply valid_link_eq with (node := (SymlinkNode sympath)) in H0; auto.
+      inversion H0.
+  + inversion H1; subst.
+    - exfalso.
+      eapply valid_link_eq with (node := (FileNode inum)) in H0; auto.
+      inversion H0.
+    -  exfalso.
+      eapply valid_link_eq with (node := (DirNode inum)) in H0; auto.
+      inversion H0.
+    - 
+      eapply valid_link_eq in H0; eauto.
+      inversion H0; subst. clear H0.
+      erewrite <- IHpath_evaluates1 with (node' := symtarget0) in H9.
+      apply IHpath_evaluates2; auto.
+      auto.
+      auto.
+Qed.
+  
+Lemma path_eval_root_eq: forall pn fs node node',
+    fs_invariant fs ->
+    path_eval_root fs pn node ->
+    path_eval_root fs pn node' ->
+    node = node'.
+Proof.
+  intros.
+  eapply path_evaluates_eq; eauto.
+Qed.
+
+Lemma path_eval_root_addlink : forall fs dirnum name dirpn n,
+  path_eval_root fs dirpn (DirNode dirnum) ->
+  does_not_exist fs dirnum name ->
+  path_eval_root (add_link dirnum n name fs) dirpn (DirNode dirnum).
+Proof.
+  unfold path_eval_root, add_link, does_not_exist in *.
+  simpl in *.
+  intros.
+  induction H.
+  + constructor.
+  + eapply PathEvalFileLink; eauto.
+    edestruct H.
+    (* validlink constructors: *)
+    - constructor; simpl.
+      apply Graph.add_spec; auto.
+    - apply ValidDot.
+    - eapply ValidDotDot.
+      apply Graph.add_spec; auto.
+      right; eauto.
+    - apply ValidDotDotRoot; auto.
+  + eapply PathEvalDirLink; eauto.
+    edestruct H.
+    - constructor; simpl.
+      apply Graph.add_spec; auto.
+    - apply ValidDot.
+    - eapply ValidDotDot.
+      apply Graph.add_spec; auto.
+      right; eauto.
+    - apply ValidDotDotRoot; auto.
+  + inversion H; subst.
+    eapply PathEvalSymlink; simpl.
+    - constructor.
+      apply Graph.add_spec.
+      eauto.
+    - apply IHpath_evaluates1; eauto.
+    - apply IHpath_evaluates2; eauto.
+Qed.
+
+Lemma valid_link_addlink_does_not_exists: forall fs dirnum name h node' node'' startdir name0,
+    name <> "." ->
+    name <> ".." ->
+    fs_invariant fs ->
+    does_not_exist fs dirnum name ->
+    valid_link fs startdir name0 node'' ->
+    valid_link (add_link dirnum (FileNode h) name fs) startdir name0 node' ->
+    valid_link fs startdir name0 node'.
+Proof.
+  intros.
+  inversion H4; subst.
+  apply Graph.add_spec in H5.
+  intuition; subst. 
+  inversion H6; subst. clear H6.
+  destruct H2.
+  eexists.
+  inversion H3; subst; eauto; try congruence.
+  apply ValidDot.
+  eapply ValidDotDot.
+  apply Graph.add_spec in H5.
+  intuition; subst; try congruence.
+  eauto.
+  eapply ValidDotDotRoot.
+  unfold add_link; simpl; auto.
+Qed.
+
+Lemma path_evaluates_addlink_does_not_exists: forall fs dirnum name h node' node'' startdir path,
+    name <> "." ->
+    name <> ".." ->
+    fs_invariant fs ->
+    does_not_exist fs dirnum name ->
+    path_evaluates fs (DirNode startdir) path node'' ->
+    path_evaluates (add_link dirnum (FileNode h) name fs) (DirNode startdir) path node' ->
+    path_evaluates fs (DirNode startdir) path node'.
+Proof.
+  intros.
+  remember ((add_link dirnum (FileNode h) name fs)).
+  generalize dependent fs.
+  generalize dependent node''.
+  induction H4; intros; subst.
+  + constructor.
+  + apply PathEvalFileLink.
+    eapply valid_link_addlink_does_not_exists in H1; eauto.
+    inversion H4; subst; eauto.
+    inversion H11; subst; eauto.
+    eapply valid_link_addlink_does_not_exists in H1; eauto.
+    eapply H2 in H1.
+    apply H1 in  H9.
+    congruence.
+  + inversion H5; subst; eauto.
+
+    eapply valid_link_addlink_does_not_exists in H1; eauto.
+
+    eapply PathEvalDirLink; eauto.
+    eapply valid_link_addlink_does_not_exists in H1; eauto.
+    eapply valid_link_eq with (node := (DirNode inum0)) in H1; eauto.
+    inversion H1; subst.
+    eapply IHpath_evaluates; eauto.
+
+    eapply valid_link_addlink_does_not_exists in H1; eauto.
+    eapply H2 in H1.
+    apply H1 in  H10.
+    congruence.
+
+  + inversion H4; subst; auto.
+    
+    eapply valid_link_addlink_does_not_exists in H1; eauto.
+    eapply H2 in H1.
+    apply H1 in  H10.
+    congruence.
+
+    eapply valid_link_addlink_does_not_exists in H1; eauto.
+    eapply H2 in H1.
+    apply H1 in  H9.
+    congruence.
+
+    eapply PathEvalSymlink; eauto.
+
+    eapply valid_link_addlink_does_not_exists in H1; eauto.
+    eapply valid_link_eq with (node := (SymlinkNode sympath0)) in H1; eauto.
+    inversion H1; subst. clear H1.
+
+    replace symtarget0 with symtarget in *; eauto.
+    eapply path_evaluates_eq; try eassumption.
+    eapply IHpath_evaluates1; eauto.
+Qed.
+
+Lemma path_eval_addlink' : forall fs startdir dirpn dirnum h name node',
+    name <> "." ->
+    name <> ".." ->
+    fs_invariant fs ->
+    does_not_exist fs dirnum name ->
+    path_evaluates fs startdir dirpn (DirNode dirnum) ->
+    path_evaluates (add_link dirnum (FileNode h) name fs) startdir dirpn node' ->
+    node' = (DirNode dirnum).
+Proof.
+  intros.
+  generalize dependent fs; intros.
+  induction H3.
+  + inversion H4; subst.
+    constructor.
+  + inversion H4; subst. clear H4.
+    eapply valid_link_addlink_does_not_exists in H8; eauto.
+    eapply valid_link_addlink_does_not_exists in H9; eauto.
+    exfalso.
+    eapply H1 in H3.
+    eapply H3 in H9.
+    congruence.
+
+    eapply valid_link_addlink_does_not_exists in H9; eauto.
+    exfalso.
+    eapply H1 in H3.
+    eapply H3 in H9.
+    congruence.
+    
+  + inversion H4; subst. clear H4.
+    eapply valid_link_addlink_does_not_exists in H11; eauto.
+    exfalso.
+    eapply H1 in H3.
+    eapply H3 in H11.
+    congruence.
+
+    eapply valid_link_addlink_does_not_exists in H10; eauto.
+    eapply H1 in H3.
+    eapply H3 in H10.
+    inversion H10; subst. clear H10.
+    apply IHpath_evaluates; eauto.
+
+    
+    eapply valid_link_addlink_does_not_exists in H10; eauto.
+    eapply H1 in H3.
+    eapply H3 in H10.
+    inversion H10.
+    
+  + inversion H4; subst. clear H4.
+    eapply valid_link_addlink_does_not_exists in H10; eauto.
+    exfalso.
+    eapply H1 in H3.
+    eapply H3 in H10.
+    congruence.
+
+    eapply valid_link_addlink_does_not_exists in H9; eauto.
+    exfalso.
+    eapply H1 in H3.
+    eapply H3 in H9.
+    congruence.
+
+    eapply valid_link_addlink_does_not_exists in H9; eauto.
+    eapply H1 in H3.
+    eapply H3 in H9. clear H3.
+    inversion H9; subst. clear H9.
+    intuition idtac.
+    apply H3.
+    replace symtarget with symtarget0; eauto.
+    eapply path_evaluates_eq. eassumption.
+    2: eassumption.
+    eapply path_evaluates_addlink_does_not_exists; eauto.
+Qed.
+
+Lemma path_eval_root_addlink' : forall fs dirnum name dirpn h node',
+    name <> "." ->
+    name <> ".." ->
+    fs_invariant fs ->
+    does_not_exist fs dirnum name ->
+    path_eval_root fs dirpn (DirNode dirnum) ->
+    path_eval_root (add_link dirnum (FileNode h) name fs) dirpn node' ->
+    path_eval_root fs dirpn node'.
+Proof.
+  unfold path_eval_root.
+  intros.
+  eapply path_eval_addlink' in H4; subst; eauto.
+Qed.
+  
+Lemma path_eval_root_updfile : forall fs dirnum h data dirpn,
+  path_eval_root fs dirpn (DirNode dirnum) ->
+  path_eval_root (upd_file h data fs) dirpn (DirNode dirnum).
+Proof.
+  intros.
+  unfold path_eval_root, upd_file; simpl.
+  induction H.
+  + constructor.
+  + eapply PathEvalFileLink; eauto.
+    edestruct H.
+    - constructor; simpl; auto.
+    - apply ValidDot.
+    - eapply ValidDotDot; simpl; eauto.
+    - apply ValidDotDotRoot; auto.
+  + eapply PathEvalDirLink; eauto.
+    edestruct H.
+    - constructor; simpl; auto.
+    - apply ValidDot.
+    - eapply ValidDotDot; simpl; eauto.
+    - apply ValidDotDotRoot; auto.
+  + eapply PathEvalSymlink; simpl.
+    inversion H. constructor. eauto.
+    apply IHpath_evaluates1; eauto.
+    apply IHpath_evaluates2; eauto.
+Qed.
+
+Lemma path_evaluates_updfile' : forall fs node h data dirpn startdir,
+  path_evaluates (upd_file h data fs) startdir dirpn node ->
+  path_evaluates fs startdir dirpn node.
+Proof.
+  intros.
   match goal with
-  | H : {| LinkFrom := ?a; LinkTo := ?b; LinkName := ?c |} =
-        {| LinkFrom := ?d; LinkTo := ?e; LinkName := ?f |} |- _ =>
-    destruct (Graph.eq_dec (mkLink a b c) (mkLink d e f)); congruence
+  | H : path_evaluates ?fs0 ?dir0 ?pn0 ?node0 |- _ =>
+    remember fs0;
+    induction H; intros; subst; simpl
   end.
+  + constructor.
+  + eapply PathEvalFileLink; eauto.
+    inversion H; clear H; subst.
+    constructor. eauto.
+  + eapply PathEvalDirLink; eauto.
+    inversion H; clear H; subst.
+    - constructor. eauto.
+    - apply ValidDot.
+    - eapply ValidDotDot; simpl; eauto.
+    - apply ValidDotDotRoot; auto.
+  + eapply PathEvalSymlink; simpl.
+    inversion H; clear H; subst.
+    constructor; eauto.
+    eapply IHpath_evaluates1; eauto.
+    apply IHpath_evaluates2; eauto.
+Qed.
 
-(** Definition of concurrent tree modifications, to write specifications *)
+Lemma path_eval_root_updfile' : forall fs node h data dirpn,
+  path_eval_root (upd_file h data fs) dirpn node ->
+  path_eval_root fs dirpn node.
+Proof.
+  intros.
+  eapply path_evaluates_updfile'; eauto.
+Qed.
 
-Definition tree_transform := Graph.t -> Graph.t.
+Lemma fs_invariant_create : forall dirnum h name fs,
+    name <> "." ->
+    name <> ".." ->
+    does_not_exist fs dirnum name ->
+    file_handle_unused fs h ->
+    file_handle_valid fs h ->
+    fs_invariant fs ->
+    fs_invariant (create_file dirnum h name fs).
+Proof.
+  unfold fs_invariant.
+  intros.
 
-Definition transform_fs (fs : FS) (xform : tree_transform) :=
-  mkFS (FSRoot fs) (xform (FSLinks fs)) (FSFiles fs).
+  unfold unique_dirents; intros.
 
-Definition add_link (srcdir : nat) (dst : Node) (name : string) : tree_transform :=
-  fun links => Graph.add (mkLink srcdir dst name) links.
+  repeat match goal with
+  | H : valid_link _ _ _ _ |- _ =>
+    inversion H; clear H; subst
+  | H : Graph.In _ _ |- _ =>
+    apply Graph.add_spec in H; intuition idtac
+  | H : mkLink _ _ _ = mkLink _ _ _ |- _ =>
+    inversion H; clear H; subst
+  | _ =>
+    solve [ exfalso; eauto ]
+  | _ =>
+    eauto
+  end.
+Qed.
 
-Definition remove_link (srcdir : nat) (dst : Node) (name : string) : tree_transform :=
-  fun links => Graph.remove (mkLink srcdir dst name) links.
+Lemma does_not_exist_addlink : forall fs dirnum name dirnum0 n0 name0,
+  does_not_exist (add_link dirnum0 n0 name0 fs) dirnum name ->
+  does_not_exist fs dirnum name.
+Proof.
+  intros.
+  unfold does_not_exist, add_link in *.
+  simpl in *.
+  intro.
+  destruct H.
+  deex.
+  eexists.
+  apply Graph.add_spec. right.
+  apply H.
+Qed.
+  
+Lemma does_not_exist_addlink_same_dirnum : forall fs dirnum name n0 name0,
+  does_not_exist fs dirnum name ->
+  name <> name0 ->
+  does_not_exist (add_link dirnum n0 name0 fs) dirnum name.
+Proof.
+  intros.
+  unfold does_not_exist, add_link in *.
+  simpl in *.
+  intro.
+  deex.
+  apply Graph.add_spec in H1.
+  intuition idtac.
+  inversion H2; congruence.
+  destruct H.
+  eexists.
+  apply H2.
+Qed.
+  
+Lemma does_not_exist_updfile : forall fs h data dirnum name,
+  does_not_exist (upd_file h data fs) dirnum name ->
+  does_not_exist fs dirnum name.
+Proof.
+  intros.
+  unfold does_not_exist, upd_file in *.
+  simpl in *; auto.
+Qed.
 
-Definition xform_both (x1 x2 : tree_transform) :=
-  fun t => x2 (x1 t).
+Lemma does_not_exist_updfile' : forall fs h data dirnum name,
+  does_not_exist fs dirnum name ->
+  does_not_exist (upd_file h data fs) dirnum name.
+Proof.
+  intros.
+  unfold does_not_exist, upd_file in *.
+  simpl in *; auto.
+Qed.
+  
+Hint Resolve does_not_exist_addlink.
+Hint Resolve does_not_exist_addlink_same_dirnum.
+Hint Resolve does_not_exist_updfile.
+Hint Resolve does_not_exist_updfile'.
 
-Definition xform_id : tree_transform :=
-  fun t => t.
+Lemma file_handle_unused_updfile : forall fs h0 data0 h,
+  file_handle_unused (upd_file h0 data0 fs) h ->
+  file_handle_unused fs h.
+Proof.
+  intros.
+  unfold file_handle_unused, upd_file in *.
+  simpl in *; auto.
+Qed.
 
-Notation "x1 ;; x2" := (xform_both x1 x2) (at level 50).
+Lemma file_handle_unused_addlink : forall fs dirnum n name h,
+  file_handle_unused (add_link dirnum n name fs) h ->
+  file_handle_unused fs h.
+Proof.
+  intros.
+  unfold file_handle_unused, add_link in *.
+  simpl in *.
+  intro.
+  repeat deex.
+  destruct H.
+  repeat eexists.
+  apply Graph.add_spec.
+  right. apply H0.
+Qed.
+  
+Lemma file_handle_unused_updfile' : forall fs h0 data0 h,
+  file_handle_unused fs h ->
+  file_handle_unused (upd_file h0 data0 fs) h.
+Proof.
+  intros.
+  unfold file_handle_unused, upd_file in *.
+  simpl in *; auto.
+Qed.
 
-(** This is what a specification looks like *)
+Lemma file_handle_unused_addlink' : forall fs dirnum n name h,
+  file_handle_unused fs h ->
+  n <> FileNode h ->
+  file_handle_unused (add_link dirnum n name fs) h.
+Proof.
+  intros.
+  unfold file_handle_unused, add_link in *.
+  simpl in *.
+  intro.
+  repeat deex.
+  apply Graph.add_spec in H1.
+  intuition idtac.
+  inversion H2; congruence.
+  destruct H.
+  repeat eexists.
+  apply H2.
+Qed.
+  
+Lemma file_handle_unused_ne : forall fs dirnum v0 v1 name,
+  file_handle_unused (add_link dirnum (FileNode v0) name fs) v1 ->
+  FileNode v1 <> FileNode v0.
+Proof.
+  intros.
+  unfold file_handle_unused, add_link in *.
+  simpl in *.
+  intro.
+  destruct H.
+  repeat eexists.
+  apply Graph.add_spec.
+  left. rewrite H0; eauto.
+Qed.
 
-Record specification (R : Type) := mkSpec {
-  Result : forall (result : R) (fs : FS), Prop;
-  AddLinks : tree_transform;
-  RemoveLinks : tree_transform;
-}.
+Hint Resolve file_handle_unused_updfile.
+Hint Resolve file_handle_unused_addlink.
+Hint Resolve file_handle_unused_addlink'.
+Hint Resolve file_handle_unused_ne.
 
-Definition spec_start {R} (fs : FS) (spec : specification R) : FS :=
-  transform_fs fs (AddLinks spec).
+Lemma file_handle_valid_updfile : forall fs h0 data0 h,
+  file_handle_valid (upd_file h0 data0 fs) h ->
+  file_handle_valid fs h.
+Proof.
+  intros.
+  unfold file_handle_valid, file_handle_valid, upd_file in *.
+  simpl in *.
+  rewrite length_list_upd in H; auto.
+Qed.
 
-Definition spec_finish {R} (fs : FS) (spec : specification R) : FS :=
-  transform_fs fs (RemoveLinks spec ;; AddLinks spec).
+Lemma file_handle_valid_addlink : forall fs dirnum n name h,
+  file_handle_valid (add_link dirnum n name fs) h ->
+  file_handle_valid fs h.
+Proof.
+  intros.
+  unfold file_handle_valid, file_handle_valid, add_link in *.
+  simpl in *; auto.
+Qed.
 
-Definition spec_ok {R} (fs : FS) (spec : specification R) (r : R) : Prop :=
-  Result spec r fs.
+Lemma file_handle_valid_updfile' : forall fs h0 data0 h,
+  file_handle_valid fs h ->
+  file_handle_valid (upd_file h0 data0 fs) h.
+Proof.
+  intros.
+  unfold file_handle_valid, file_handle_valid, upd_file in *.
+  simpl in *.
+  rewrite length_list_upd; auto.
+Qed.
+  
+Lemma file_handle_valid_addlink' : forall fs dirnum n name h,
+  file_handle_valid fs h ->
+  file_handle_valid (add_link dirnum n name fs) h.
+Proof.
+  intros.
+  unfold file_handle_valid, file_handle_valid, add_link in *.
+  simpl in *; auto.
+Qed.
+  
+Hint Resolve file_handle_valid_updfile.
+Hint Resolve file_handle_valid_addlink.
+Hint Resolve file_handle_valid_updfile'.
+Hint Resolve file_handle_valid_addlink'.
+
+Lemma valid_link_updfile' : forall fs h data dir name target,
+  valid_link (upd_file h data fs) dir name target ->
+  valid_link fs dir name target.
+Proof.
+  intros.
+  remember (upd_file h data fs); generalize dependent fs.
+  induction H; intros; subst.
+  - constructor. eauto.
+  - eapply ValidDot.
+  - eapply ValidDotDot. eauto.
+  - eapply ValidDotDotRoot. eauto.
+Qed.
+
+(* File system operations *)
+
+Inductive stat_result :=
+| StatMissing
+| StatFile
+| StatDir.
+
+Inductive fsOpT : Type -> Type :=
+| Create (dir : Pathname) (name : string) : fsOpT nat
+| Mkdir (dir : Pathname) (name : string) : fsOpT nat
+| Delete (pn : Pathname) : fsOpT unit
+| Rmdir (pn : Pathname) : fsOpT unit
+| Stat (dir : Pathname) (name : string) : fsOpT stat_result
+| Readdir (pn : Pathname) : fsOpT (list string)
+| Rename (src : Pathname) (dstdir : Pathname) (dstname : string) : fsOpT unit
+| Read (pn : Pathname) : fsOpT string
+| Write (pn : Pathname) (data : string) : fsOpT unit
+| FindAvailableName (dir : Pathname) : fsOpT string
+| Debug (s : string) : fsOpT unit.
 
 
-(** Concrete specifications *)
+(* Semantics of file system operations *)
 
-Definition lookup_spec (pn : Pathname) : specification (option Node) := {|
-  Result := fun result fs =>
-    (exists node, result = Some node /\ path_eval_root fs pn node) \/
-    result = None /\ ~ exists node, path_eval_root fs pn node;
-  AddLinks := xform_id;
-  RemoveLinks := xform_id;
-|}.
+Definition State := FS.
 
-Definition rename_overwrite_spec srcdir srcname node dstdir dstname oldnode := {|
-  Result := fun r _ => r = tt;
-  AddLinks := add_link dstdir node dstname;
-  RemoveLinks := remove_link srcdir node srcname;;
-                 remove_link dstdir oldnode dstname
-|}.
+Section StepXform.
 
-Definition rename_nonexist_spec srcdir srcname node dstdir dstname := {|
-  Result := fun r _ => r = tt;
-  AddLinks := add_link dstdir node dstname;
-  RemoveLinks := remove_link srcdir node srcname
-|}.
+  Variable opT : Type -> Type.
+  Variable op_step : OpSemantics opT State.
+  Variable EquivR : Relation_Definitions.relation State.
 
-(**
-  TODO: take just Pathname arguments, rather than relying on knowing
-  node (and oldnode, if exists) already.
+  Inductive equiv_step : OpSemantics opT State :=
+  | StepEquiv : forall `(op : opT T) tid s0 s1 s1' r,
+    op_step op tid s0 r s1' ->
+    EquivR s1 s1' ->
+    equiv_step op tid s0 r s1.
 
-  tricky issues:
-  - moving a symlink: need to move the SymlinkNode, not the evaluated target.
-  - overwriting a symlink?
-  - what if there are multiple possibilities for a given name?
-    saying "~ exists .., path_eval_root" seems to imply NONE of
-    these concurrent syscalls can be running now.
- *)
+End StepXform.
+
+Inductive fs_step : forall T, fsOpT T -> nat -> State -> T -> State -> Prop :=
+| StepCreateAt : forall dir dirnum name tid s h s',
+  path_eval_root s dir (DirNode dirnum) ->
+  does_not_exist s dirnum name ->
+  file_handle_unused s h ->
+  file_handle_valid s h ->
+  s' = create_file dirnum h name s ->
+  fs_step (Create dir name) tid s h s'
 
 (*
-Definition rename_spec srcdir srcname dstdir dstname := {|
-  Result := fun r _ =>
-    r = true <-> exists n, path_eval_root fs (srcdir ++ [srcname]) n /\
-      ~ exists d, path_eval_root fs (dstdir ++ [dstname]) (DirNode d);
-  AddLinks := add_link 
-|}.
+
+| StepMkdir : forall dir name tid s h s' dirnum newdirnum,
+  frame_pre_post s s'
+    (dir |-> Dir dirnum * (dir ++ [name]) |-> Missing)
+    (dir |-> Dir dirnum * (dir ++ [name]) |-> Dir newdirnum
+                        * subtree_pred (dir ++ [name]) empty_dir) ->
+  fs_step (Mkdir dir name) tid s h s'
+
+| StepDelete : forall pn h f tid s s',
+  frame_pre_post s s'
+    (pn |-> File h f)
+    (pn |-> Missing) ->
+  fs_step (Delete pn) tid s tt s'
+
+| StepRmdir : forall pn dirnum tid s s',
+  frame_pre_post s s'
+    (pn |-> Dir dirnum * subtree_pred pn empty_dir)
+    (pn |-> Missing) ->
+  fs_step (Rmdir pn) tid s tt s'
+
+| StepStat : forall dir name tid s r F dirnum,
+  s  |= F * dir |-> Dir dirnum ->
+  (r = StatFile ->
+    exists F' h f, F' * (dir ++ [name]) |-> File h f ===> F) ->
+  (r = StatDir ->
+    exists F' dirnum', F' * (dir ++ [name]) |-> Dir dirnum' ===> F) ->
+  (r = StatMissing ->
+    exists F', F' * (dir ++ [name]) |-> Missing ===> F) ->
+  fs_step (Stat dir name) tid s r s
+
+| StepReaddir : forall dir tid s r F dirnum,
+  s  |= F * dir |-> Dir dirnum ->
+  (forall fn,
+    (In fn r /\ exists F' handle f,
+     F' * (dir ++ [fn]) |-> File handle f ===> F) \/
+    (In fn r /\ exists F' dirinum,
+     F' * (dir ++ [fn]) |-> Dir dirinum ===> F) \/
+    (~ In fn r /\ exists F',
+     F' * (dir ++ [fn]) |-> Missing ===> F)) ->
+  fs_step (Readdir dir) tid s r s
+
+| StepRename : forall src dstdir dstname tid s handle f s' dirnum,
+  frame_pre_post s s'
+    (src |-> File handle f
+          * dstdir |-> Dir dirnum
+          * (dstdir ++ [dstname]) |-> Missing)
+    (src |-> Missing
+          * dstdir |-> Dir dirnum
+          * (dstdir ++ [dstname]) |-> File handle f) ->
+  fs_step (Rename src dstdir dstname) tid s tt s'
+
+| StepRead : forall pn tid s r handle F,
+  s  |= F * pn |-> File handle r ->
+  fs_step (Read pn) tid s (FileData r) s
+
+| StepWrite : forall pn tid s s' handle f0 data,
+  frame_pre_post s s'
+    (pn |-> File handle f0)
+    (pn |-> File handle (mk_file data)) ->
+  fs_step (Write pn data) tid s tt s'
+
+| StepFindAvailableName : forall dir dirnum tid s name F,
+  starts_with_tid tid name ->
+  s  |= F * dir |-> Dir dirnum * (dir ++ [name]) |-> Missing ->
+  fs_step (FindAvailableName dir) tid s name s
+
+| StepDebug : forall msg tid s,
+  fs_step (Debug msg) tid s tt s
 *)
+.
 
-Definition names := list string.
+Hint Constructors fs_step.
 
-Definition dirents dirnum (g: Graph.t) :=
-  Graph.filter (fun (l: Link) => (beq_nat (LinkFrom l) dirnum)) g.
+Definition fs_step_equiv : OpSemantics fsOpT State :=
+  equiv_step fs_step FSEquiv.
 
-Definition dirnames dirnum g : names :=
-  let dir := dirents dirnum g in
-  map (fun (l:Link) => (LinkName l)) (Graph.elements dir).
+Instance fs_step_equiv_proper :
+  Proper (eq ==> eq ==> eq ==> eq ==> FSEquiv ==> iff) (@fs_step_equiv T).
+Proof.
+  intros.
+  intros ? ? ?; subst.
+  intros ? ? ?; subst.
+  intros fs1 fs1' ?.
+  intros ? ? ?; subst.
+  intros fs2 fs2' ?.
+  unfold fs_step_equiv; intuition.
+  - inversion H0; clear H0; repeat sigT_eq.
+    econstructor; eauto.
+    etransitivity; eauto.
+      symmetry; eauto.
+  - inversion H0; clear H0; repeat sigT_eq.
+    econstructor; eauto.
+    etransitivity; eauto.
+Qed.
 
-Definition readdir_spec pn : specification (option names)  := {|
-  Result := fun result fs =>
-              (exists node dir n, dir = Some (DirNode n) /\ path_eval_root fs pn node /\
-                           result = Some (dirnames n (FSLinks fs))
-              ) \/
-              result = None /\  ~ exists node n, path_eval_root fs pn node /\ node = (DirNode n);
-  AddLinks := xform_id;
-  RemoveLinks := xform_id;
-|}.
+Instance file_handle_unused_proper :
+  Proper (FSEquiv ==> eq ==> iff) file_handle_unused.
+Proof.
+  intros ? ? ?; subst.
+  intros ? ? ?; subst.
+  unfold FSEquiv in H.
+  unfold file_handle_unused; intuition; repeat deex.
+  - apply H2 in H3. eauto.
+  - apply H2 in H3. eauto.
+Qed.
+
+Instance file_handle_valid_proper :
+  Proper (FSEquiv ==> eq ==> iff) file_handle_valid.
+Proof.
+  intros ? ? ?; subst.
+  intros ? ? ?; subst.
+  unfold FSEquiv in H.
+  unfold file_handle_valid; intuition; congruence.
+Qed.
+
+Instance does_not_exist_proper :
+  Proper (FSEquiv ==> eq ==> eq ==> iff) does_not_exist.
+Proof.
+  intros ? ? ?; subst.
+  intros ? ? ?; subst.
+  intros ? ? ?; subst.
+  unfold FSEquiv in H.
+  unfold does_not_exist; intuition; repeat deex.
+  - apply H2 in H3. eauto.
+  - apply H2 in H3. eauto.
+Qed.
+
+Instance FSEquiv_proper :
+  Proper (FSEquiv ==> FSEquiv ==> iff) FSEquiv.
+Proof.
+  intros ? ? ?; subst.
+  intros ? ? ?; subst.
+  rewrite H. rewrite H0. reflexivity.
+Qed.
+
+Instance upd_file_proper :
+  Proper (eq ==> eq ==> FSEquiv ==> FSEquiv) upd_file.
+Proof.
+  intros ? ? ?; subst.
+  intros ? ? ?; subst.
+  intros ? ? ?; subst.
+  unfold upd_file.
+  unfold FSEquiv in *.
+  intuition; simpl.
+  rewrite H; eauto.
+Qed.
+
+Instance add_link_proper :
+  Proper (eq ==> eq ==> eq ==> FSEquiv ==> FSEquiv) add_link.
+Proof.
+  intros ? ? ?; subst.
+  intros ? ? ?; subst.
+  intros ? ? ?; subst.
+  intros ? ? ?; subst.
+  unfold add_link.
+  unfold FSEquiv in *.
+  intuition; simpl.
+
+  unfold Graph.Equal; split; intros; apply Graph.add_spec.
+  - apply Graph.add_spec in H1; intuition; subst.
+    apply H2 in H3. eauto.
+  - apply Graph.add_spec in H1; intuition; subst.
+    apply H2 in H3. eauto.
+Qed.
+
+Instance create_file_proper :
+  Proper (eq ==> eq ==> eq ==> FSEquiv ==> FSEquiv) create_file.
+Proof.
+  intros ? ? ?; subst.
+  intros ? ? ?; subst.
+  intros ? ? ?; subst.
+  intros ? ? ?; subst.
+  unfold create_file.
+  rewrite H.
+  reflexivity.
+Qed.
+
+Instance fs_invariant_proper :
+  Proper (FSEquiv ==> iff) fs_invariant.
+Proof.
+  intros ? ? ?; subst.
+  unfold fs_invariant, unique_dirents; intuition.
+  - rewrite <- H in *.
+    eauto.
+  - rewrite H in *.
+    eauto.
+Qed.
 
